\documentclass{paper}

%% Set page size and margins
\usepackage[a4paper,margin=2cm]{geometry}

\usepackage[utf8]{inputenc}
\usepackage[T1]{fontenc}
\usepackage{amsmath}
\usepackage{amssymb}
\usepackage{ctex}
\usepackage{graphicx}
\usepackage{multicol}
\usepackage{listings}
\setlength{\columnsep}{1pt}

%% Set code style
\definecolor{codegreen}{rgb}{0,0.6,0}
\definecolor{codegray}{rgb}{0.5,0.5,0.5}
\definecolor{codepurple}{rgb}{0.58,0,0.82}
\definecolor{backcolour}{rgb}{0.96,0.96,0.96}

\lstdefinestyle{mystyle}{
    backgroundcolor=\color{backcolour},   
    commentstyle=\color{codegreen},
    keywordstyle=\color{magenta},
    numberstyle=\tiny\color{codegray},
    stringstyle=\color{codepurple},
    basicstyle=\ttfamily\footnotesize,
    breakatwhitespace=false,         
    breaklines=true,                 
    captionpos=b,                    
    keepspaces=true,                 
    numbers=left,                    
    numbersep=5pt,                  
    showspaces=false,                
    showstringspaces=false,
    showtabs=false,                  
    tabsize=2
}

\lstset{style=mystyle}

\title{Derivation of pLSA}
\author{CanoY}

\begin{document}
\maketitle
Derive the Co-occurrence Model of pLSA using EM algorithm.\\
\textbf{Prove:}
    \begin{align*}
        L&=\prod\limits_{i=1}^M \prod\limits_{j=1}^N P(w_i, d_j)^{n(w_i,d_j)}\\
        LL&=\sum_i \sum_j n(w_i,d_j)\log P(w_i,d_j)\\
        &=\sum_i \sum_j n(w_i,d_j)\log \sum\limits_{k=1}^K P(w_i,d_j,z_k)
    \end{align*}
\textbf{E step:}
    \begin{align*}
        LL&\geq \sum_i \sum_j n(w_i,d_j) \sum_k P^{(t+1)}(z_k\vert w_i,d_j) \log P(w_i,d_j,z_k)\\
        P^{(t+1)}(z_k\vert w_i,d_j) &= \frac{
                P^{(t)}(w_i\vert z_k) P^{(t)}(d_j\vert z_k) P^{(t)}(z_k)
            }{
                \sum_k P^{(t)}(w_i\vert z_k) P^{(t)}(d_j\vert z_k) P^{(t)}(z_k)
            }
    \end{align*}
\textbf{M step:}
    \begin{align*}
        \min\quad&P:=\sum_i \sum_j n(w_i,d_j) \sum_k P^{(t+1)}(z_k\vert w_i,d_j) \log [P(z_k) P(w_i\vert z_k) P(d_j\vert z_k)]\\
        \text{s.t.}\quad&\sum_i P(w_i\vert z_k)=1,\quad z=1,2,3,\cdots,K\\
        \quad&\sum_j P(d_j\vert z_k)=1,\quad z=1,2,3,\cdots,K\\
        \quad&\sum_i P(z_k)=1
    \end{align*}
    \begin{align*}
        \Lambda &= P + \sum_k u_k(\sum_i P(w_i\vert z_k)-1) +
        \sum_k v_k(\sum_j P(d_j\vert z_k)-1) +
        \lambda(\sum_k P(z_k)-1)\\
        \frac{\partial \Lambda}{\partial P(z_k)} &=\frac{\sum_i\sum_j n(w_i,d_j)P^{(t+1)}(z_k\vert w_i,d_j)}{P(z_k)}+\lambda = 0\\
        & \underline{\Rightarrow P^{(t+1)}(z_k) = \dfrac{R_k}{N_w}}\\
        & R_k = \sum_i\sum_j n(w_i,d_j)P^{(t+1)}(z_k\vert w_i,d_j), \quad N_w =\sum_i\sum_j n(w_i,d_j)\\
        \frac{\partial \Lambda}{\partial P(w_i\vert z_k)}&=\frac{\sum_j n(w_i,d_j)P^{(t+1)}(z_k\vert w_i,d_j)}{P(w_i\vert z_k)}+u_k=0\\
        & \underline{\Rightarrow P^{(t+1)}(w_i\vert z_k) = \dfrac{R_{ik}}{R_k}}\\
        & R_{ik} = \sum_j n(w_i,d_j)P^{(t+1)}(z_k\vert w_i,d_j)\\
        \frac{\partial \Lambda}{\partial P(d_j\vert z_k)}&=\frac{\sum_i n(w_i,d_j)P^{(t+1)}(z_k\vert w_i,d_j)}{P(d_j\vert z_k)}+v_k=0\\
        & \underline{\Rightarrow P^{(t+1)}(w_i\vert z_k) = \dfrac{R_{jk}}{R_k}}\\
        & R_{jk} = \sum_i n(w_i,d_j)P^{(t+1)}(z_k\vert w_i,d_j)
    \end{align*}
\end{document}